AczelSetTheory/Axioms/Replacement.lean
@@ -59,7 +59,7 @@ theorem image_subset_range
 
 /-- Si f es función y x ∈ A ∩ domain f, entonces apply f x ∈ image f A. -/
 theorem apply_mem_image
-  (f A x : HFSet) (hf : isFunction f) (hxA : x ∈ A) (hx : ∃ b, ⟪x, b⟫ ∈ f) :
+  (f A x : HFSet) (_hf : isFunction f) (hxA : x ∈ A) (hx : ∃ b, ⟪x, b⟫ ∈ f) :
     apply f x hx ∈ image f A
       := by
   rw [mem_image]
