test_q.lean
@@ -1,0 +1,6 @@
+import AczelSetTheory.HFSets
+example : HFSet.repr HFSet.empty = CList.empty := by
+  unfold HFSet.repr HFSet.empty
+  change CList.normalize CList.empty = CList.empty
+  unfold CList.normalize CList.empty
+  simp [CList.dedup, CList.dedupAux, CList.insertionSort]
